Lib/Extra.v
@@ -1,0 +1,7 @@
+(* Complements to the standard Coq library and ssreflect *)
+
+Require Import Coq.ZArith.ZArith.
+From mathcomp Require Import ssreflect ssrfun ssrbool eqtype.
+
+Definition Z_eqMixin := EqMixin Z.eqb_spec.
+Canonical Z_eqType := Eval hnf in EqType Z Z_eqMixin.
